Fixing simulation statement (#60)
Update simulation relation, enabling almost full proof of adversarial non-interference.  Just need to handle message forwarding.

KeyManagement/Simulation.v
@@ -191,39 +191,41 @@ Definition adv_universe_ok {A B} (U : RealWorld.universe A B) : Prop :=
     /\ adv_no_honest_keys honestk U.(RealWorld.adversary).(RealWorld.key_heap).
 
 Section Simulation.
-  Variable A : Type.
+  Variable A B : Type.
+  Variable advP : RealWorld.user_data B -> Prop.
   Variable R : RealWorld.simpl_universe A -> IdealWorld.universe A -> Prop.
 
   Definition simulates_silent_step :=
-    forall B (b : B) (U__r : RealWorld.universe A B) U__i,
+    forall (U__r : RealWorld.universe A B) U__i,
     R (RealWorld.peel_adv U__r) U__i
     -> universe_ok U__r
     -> adv_universe_ok U__r
+    -> advP U__r.(RealWorld.adversary)
     -> forall U__r',
         rstepSilent U__r U__r'
         -> exists U__i',
           istepSilent ^* U__i U__i'
-        /\ universe_ok U__r'
         /\ R (RealWorld.peel_adv U__r') U__i'.
 
   Definition simulates_labeled_step :=
-    forall B (b : B) (U__r : RealWorld.universe A B) U__i,
+    forall (U__r : RealWorld.universe A B) U__i,
     R (RealWorld.peel_adv U__r) U__i
     -> universe_ok U__r
     -> adv_universe_ok U__r
+    -> advP U__r.(RealWorld.adversary)
     -> forall a1 U__r',
         RealWorld.step_universe U__r (Action a1) U__r' (* excludes adversary steps *)
         -> exists a2 U__i' U__i'',
           istepSilent^* U__i U__i'
         /\ IdealWorld.lstep_universe U__i' (Action a2) U__i''
         /\ action_matches a1 a2
-        /\ R (RealWorld.peel_adv U__r') U__i''
-        /\ universe_ok U__r'.
+        /\ R (RealWorld.peel_adv U__r') U__i''.
 
   Definition simulates_universe_ok :=
     forall B (U__r : RealWorld.universe A B) U__i,
       R (strip_adversary U__r) U__i
       -> universe_ok U__r
+      -> adv_universe_ok U__r
       -> forall U__r' lbl,
         RealWorld.step_universe U__r lbl U__r'
         -> universe_ok U__r'.
@@ -238,7 +240,7 @@ Section Simulation.
            U__r.(RealWorld.all_ciphers)
            a.
 
-  Definition simulates {B} (U__r : RealWorld.universe A B) (U__i : IdealWorld.universe A) :=
+  Definition simulates (U__r : RealWorld.universe A B) (U__i : IdealWorld.universe A) :=
 
     (* conditions for simulation steps *)
     simulates_silent_step
@@ -253,47 +255,113 @@ Section Simulation.
 
 End Simulation.
 
-Definition refines {A B : Type} (U1 : RealWorld.universe A B)(U2 : IdealWorld.universe A) :=
-  exists R, simulates R U1 U2.
+Definition refines {A B : Type} (advP : RealWorld.user_data B -> Prop) (U1 : RealWorld.universe A B) (U2 : IdealWorld.universe A) :=
+  exists R, simulates advP R U1 U2.
 
-Infix "<|" := refines (no associativity, at level 70).
+(* Notation "x <- c1 ; c2" := (Bind c1 (fun x => c2)) (right associativity, at level 75) : realworld_scope. *)
 
-Lemma msgCiphersSigned_addnl_cipher :
-  forall cs msgs honestk c_id c,
-    Forall (RealWorld.msgCipherOk honestk cs) msgs
-    -> ~ In c_id cs
-    -> Forall (RealWorld.msgCipherOk honestk (cs $+ (c_id,c))) msgs.
-Proof.
-  induction msgs; intros; econstructor; invert H; eauto; clean_map_lookups.
-  unfold RealWorld.msgCipherOk in H3. unfold RealWorld.msgCipherOk.
-  destruct a; intuition idtac.
-  destruct m; eauto.
-  - invert H1; invert H2; repeat eexists.
-    destruct (c_id ==n msg_id); subst; clean_map_lookups; eauto.
-  - destruct (c_id ==n sig); subst; clean_map_lookups; eauto.
-Qed.
+Notation "u1 <| u2 / p " := (refines p u1 u2) (no associativity, at level 70).
 
-Lemma encrypted_cipher_ok_addnl_cipher :
-  forall honestk cs c_id c1 c2,
-    encrypted_cipher_ok honestk cs c1
-    -> ~ In c_id cs
-    -> encrypted_cipher_ok honestk (cs $+ (c_id,c2)) c1.
-Proof.
-  inversion 1; intros; try solve [ econstructor; eauto ].
-  - econstructor; eauto.
-    eapply msgCiphersSigned_addnl_cipher; auto.
-  - eapply SigEncCipherHonestSignedEncKeyHonestOk; eauto.
-    eapply msgCiphersSigned_addnl_cipher; auto.
-Qed.
+Definition lameAdv {B} (b : B) :=
+  fun adv => adv.(RealWorld.protocol) = RealWorld.Return b.
 
-Lemma encrypted_ciphers_ok_addnl_cipher :
-  forall honestk cs c_id c,
-    Forall_natmap (encrypted_cipher_ok honestk cs) cs
-    -> ~ In c_id cs
-    -> Forall_natmap (encrypted_cipher_ok honestk (cs $+ (c_id, c))) cs.
-Proof.
-  intros.
-  rewrite Forall_natmap_forall in *.
-  intros.
-  specialize (H _ _ H1); eauto using encrypted_cipher_ok_addnl_cipher.
-Qed.
+Definition awesomeAdv : forall B, RealWorld.user_data B -> Prop :=
+  fun _ _ => True.
+
+
+Section RealWorldLemmas.
+
+  Import RealWorld.
+
+  Lemma msgCiphersSigned_addnl_cipher :
+    forall cs msgs honestk c_id c,
+      Forall (RealWorld.msgCipherOk honestk cs) msgs
+      -> ~ In c_id cs
+      -> Forall (RealWorld.msgCipherOk honestk (cs $+ (c_id,c))) msgs.
+  Proof.
+    induction msgs; intros; econstructor; invert H; eauto; clean_map_lookups.
+    unfold RealWorld.msgCipherOk in H3. unfold RealWorld.msgCipherOk.
+    destruct a; intuition idtac.
+    destruct m; eauto.
+    - invert H1; invert H2; repeat eexists.
+      destruct (c_id ==n msg_id); subst; clean_map_lookups; eauto.
+    - destruct (c_id ==n sig); subst; clean_map_lookups; eauto.
+  Qed.
+
+  Lemma encrypted_cipher_ok_addnl_cipher :
+    forall honestk cs c_id c1 c2,
+      encrypted_cipher_ok honestk cs c1
+      -> ~ In c_id cs
+      -> encrypted_cipher_ok honestk (cs $+ (c_id,c2)) c1.
+  Proof.
+    inversion 1; intros; try solve [ econstructor; eauto ].
+    - econstructor; eauto.
+      eapply msgCiphersSigned_addnl_cipher; auto.
+    - eapply SigEncCipherHonestSignedEncKeyHonestOk; eauto.
+      eapply msgCiphersSigned_addnl_cipher; auto.
+  Qed.
+
+  Lemma encrypted_ciphers_ok_addnl_cipher :
+    forall honestk cs c_id c,
+      Forall_natmap (encrypted_cipher_ok honestk cs) cs
+      -> ~ In c_id cs
+      -> Forall_natmap (encrypted_cipher_ok honestk (cs $+ (c_id, c))) cs.
+  Proof.
+    intros.
+    rewrite Forall_natmap_forall in *.
+    intros.
+    specialize (H _ _ H1); eauto using encrypted_cipher_ok_addnl_cipher.
+  Qed.
+
+  Hint Resolve
+       encrypted_ciphers_ok_addnl_cipher.
+
+  Lemma adv_step_encrypted_ciphers_ok :
+    forall {A B C} cs cs' lbl (usrs usrs' : honest_users A) (adv adv' : user_data B)
+              gks gks' ks ks' qmsgs qmsgs' mycs mycs' bd bd',
+      step_user lbl None bd bd'
+      -> forall (cmd : user_cmd C) honestk,
+        bd = (usrs, adv, cs, gks, ks, qmsgs, mycs, cmd)
+        -> honestk = findUserKeys usrs
+        -> ks = adv.(key_heap)
+        -> adv_no_honest_keys honestk ks
+        -> encrypted_ciphers_ok honestk cs
+        -> forall cmd' honestk',
+            bd' = (usrs', adv', cs', gks', ks', qmsgs', mycs', cmd')
+            -> honestk' = findUserKeys usrs'
+            -> encrypted_ciphers_ok honestk' cs'.
+  Proof.
+    induction 1; inversion 1; inversion 5; intros; subst;
+      eauto 2; autorewrite with find_user_keys; eauto.
+
+    - econstructor; eauto.
+      assert (adv_no_honest_keys (findUserKeys usrs') (key_heap adv')) as ADV by assumption.
+      specialize (H20 k__signid).
+      econstructor; eauto.
+      + unfold not; intros; split_ors; split_ands; contra_map_lookup; contradiction.
+      + intros.
+        specialize (H4 _ _ H6).
+        specialize (ADV k); unfold not; intros; split_ors; split_ands; contra_map_lookup; contradiction.
+
+    - econstructor; eauto.
+      specialize (H16 k_id).
+      eapply SigCipherNotHonestOk; unfold not; intros; split_ors; split_ands; contra_map_lookup; contradiction.
+  Qed.
+
+  Lemma universe_ok_adv_step :
+    forall {A B} (U__r : universe A B) lbl usrs adv cs gks ks qmsgs mycs cmd,
+      universe_ok U__r
+      -> adv_universe_ok U__r
+      -> step_user lbl None
+                  (users U__r, adversary U__r, all_ciphers U__r, all_keys U__r,
+                   key_heap (adversary U__r), msg_heap (adversary U__r),
+                   c_heap (adversary U__r), protocol (adversary U__r)) (usrs, adv, cs, gks, ks, qmsgs, mycs, cmd)
+      -> universe_ok
+          (buildUniverseAdv
+             usrs cs gks
+             {| key_heap := ks; protocol := cmd; msg_heap := qmsgs; c_heap := mycs |}).
+  Proof.
+    unfold universe_ok, adv_universe_ok; destruct U__r; simpl; intros; split_ands; eauto using adv_step_encrypted_ciphers_ok.
+  Qed.
+
+End RealWorldLemmas.
